@base <http://folia.science.ru.nl/setdefinition#> .
@prefix rdfs: <http://www.w3.org/2000/01/rdf-schema#> .
@prefix rdf: <http://www.w3.org/1999/02/22-rdf-syntax-ns#> .
@prefix xsd: <http://www.w3.org/2001/XMLSchema#> .

# base class

:Set
    a rdf:Class ;
    rdfs:label "FoLiA Set Definition" ;
    rdfs:comment "Defines a set or taxonomy of classes for a particular linguistic annotation. These are in turn referenced by FoLiA documents." .

# set type (open/mixed/closed)

:OpenSet
    a :Set ;
    rdfs:label "open" ;
    rdfs:comment "Open set definition. Classes may refer to anything." .

:MixedSet
    a :Set ;
    rdfs:label "mixed" ;
    rdfs:comment "Mixed set definition. Classes may refer to those defined in the set definition, but open classes are also allowed." .


:ClosedSet
    a :Set ;
    rdfs:label "closed" ;
    rdfs:comment "Closed set definition. Classes must be defined in the set definition." .

:EmptySet
    a :Set ;
    rdfs:label "empty" ;
    rdfs:comment "Empty set definition. The set itself takes no classes, it may however still define subsets." .


# class  properties

:Class
    a rdf:Class ;
    rdfs:label "FoLiA Class" ;
    rdfs:comments "Defines a class in a set, a class corresponds for instance to a tag in a linguistic tagset" .

:label
    a rdf:Property ;
    rdfs:subPropertyOf rdfs:label .
    rdfs:label "The human readable label for the Set or Class"

:id
    a rdf:Property ;
    rdfs:label "ID identifying the class (or set as a whole), a class is identified by this ID or its full URI. The ID must be unique in the (sub)set." ;
    rdfs:range xsd:string .

:conceptLink
    a rdf:Property ;
    rdfs:label "Concept Link" ;
    rdfs:comment "Links a class or set to any other resource that is considered to cover the same concept" ;
    rdfs:range rdfs:Resource .


:memberOf
    a rdf:Property ;
    rdfs:label "Member of set" ;
    rdfs:comment "Each class must state what set it is a direct member of" ;
    rdfs:domain :Class ;
    rdfs:target :Set .


# class hierarchy

:parentClass
    a rdf:Property ;
    rdfs:label "Parent class" ;
    rdfs:comment "This property is used to define a taxonomy/hierarchy of classes, rather than a flat set." ;
    rdfs:domain :Class ;
    rdfs:target :Class .

# class order

:orderIndex
    a rdf:Property ;
    rdfs:domain :Class ;
    rdfs:range xsd:integer ;

# subsets

:subsetOf
    a rdf:Property ;
    rdfs:label "Subset" ;
    rdfs:comment "Sets may be nested, subsets are always referenced in the FoLiA document using 'features'" ;
    rdfs:domain :Set ;
    rdfs:target :Set .


#constraints (needs work still)

:constrain
    a rdf:Property ;
    rdfs:label "Contrain" ;
    rdfs:comment "Constrain a class from a subset to require or forbid co-occuring with another class" ;
    rdfs:domain :Class ;
    rdfs:range :Constraint .


:Constraint
    a rdf:Class ;
    rdfs:label "Constraint" ;

:ConstraintType
    a rdf:class ;
    rdfs:label "Constraint Type" ;

:Required
    a :ConstraintType .

:Forbidden
    a :ConstraintType .




